Redefine MLang

io/MLang.fst
@@ -4,13 +4,37 @@ open FStar.Tactics
 open FStar.Tactics.Typeclasses
 
 open Common
-open MIO
 
-(** ** Mlang **)
+noeq type monad = {
+  m    : Type u#a -> Type u#(max 1 a);
+  ret  : #a:Type -> a -> m a;
+  (* TODO: bind should be polymorphic in two universes *)
+  bind : #a:Type u#a -> #b:Type u#a -> m a -> (a -> m b) -> m b;
+  (* We don't want acts to be part of this monad because we want to provide different versions *)
+}
 
-effect MIIO (a:Type) = IIO.IIOwp a (Hist.trivial_hist)
+val free : monad
+let free = { 
+  m = IO.Sig.iio; 
+  ret = IO.Sig.iio_return; 
+  bind = IO.Sig.iio_bind; 
+}
 
-class mlang (t:Type) = { mldummy : unit }
+type acts (mon:monad) = op:(Universe.raise_t IO.Sig.io_cmds) -> arg:IO.Sig.io_sig.args (Universe.downgrade_val op) -> mon.m (IO.Sig.io_sig.res (Universe.downgrade_val op) arg)
+
+(** **** Free Actions **)
+val free_acts : acts free
+let free_acts cmd arg = IO.Sig.Call.iio_call (Universe.downgrade_val cmd) arg
+
+let spec_free_acts (ca:acts free) =
+  (forall (cmd:IO.Sig.io_cmds) (arg:IO.Sig.io_sig.args cmd). IO.Sig.iio_wps cmd arg `Hist.hist_ord` IIO.dm_iio_theta (ca (Universe.raise_val cmd) arg))
+
+let lemma_free_acts () : Lemma (spec_free_acts free_acts) = 
+  assert (forall (cmd:IO.Sig.io_cmds) (arg:IO.Sig.io_sig.args cmd). IO.Sig.iio_wps cmd arg `Hist.hist_ord` IIO.dm_iio_theta (free_acts (Universe.raise_val cmd) arg));
+  assert (spec_free_acts free_acts) by (assumption ())
+
+(** ** MLang **)
+class mlang (t:Type u#a) = { mldummy : unit }
 
 (** *** FO instances **)
 instance mlang_unit : mlang unit = { mldummy = () }
@@ -23,47 +47,61 @@ instance mlang_pair t1 t2 {| d1:mlang t1 |} {| d2:mlang t2 |} : mlang (t1 * t2) 
 instance mlang_either t1 t2 {| d1:mlang t1 |} {| d2:mlang t2 |} : mlang (either t1 t2) =
   { mldummy = () }
 
-instance mlang_resexn t1 {| d1:mlang t1 |} : mlang (resexn t1) =
+instance mlang_free_arrow #t1 #t2 (d1:mlang t1) (d2:mlang t2) : mlang (t1 -> free.m t2) =
   { mldummy = () }
 
-instance mlang_arrow #t1 #t2 (d1:mlang t1) (d2:mlang t2) : mlang (t1 -> MIIO (resexn t2)) =
+instance mlang_effectpoly 
+  (#ct:(Type->Type)->Type)
+  (d1:mlang (ct free.m)) : 
+  mlang (mon:monad -> acts mon -> ct mon.m) =
   { mldummy = () }
 
-open IO.Sig
-open TC.Monitorable.Hist
 
-let rec special_tree
-  (pi : monitorable_prop)
-  (tree : iio 'a) : Type0 =
-  match tree with
-  | Return _ -> True
-  | PartialCall _ _ -> False
-  | Call GetTrace arg k -> False
-  | Call cmd arg k -> forall res. special_tree pi (k res)
-  | Decorated dec m k ->
-    (forall h lt. dec h lt ==> enforced_locally pi h lt) /\
-    (forall res. special_tree pi (k res))
 
-(** this diff is problematic because it allows to use Decorated node.
-Decorated nodes come as input, but in the same time the predicate enables
-writing bad stuff **)
-type unverified_arrow (t1 t2:Type) pi =
-  f:(t1 -> MIIO (resexn t2)){forall x. special_tree pi (reify (f x))} 
+(** *** Manual tests *)
+(** Manual tests of MLang. 
+    Types of programs that should be part of MLang:
+   - [v] int -> free.m int
+   - [ ] int -> free.m (int -> free.m int)
+   - [v] (int -> free.m int) -> free.m int (?)
+   - [v] mon:monad -> acts mon -> int -> mon.m int 
+   - [v] mon:monad -> acts mon -> (int -> mon.m int) -> mon.m int 
+   - [ ] mon:monad -> acts mon -> int -> mon.m (int -> mon.m int)
+   - [v] (mon:monad -> acts mon -> int -> mon.m int) -> free.m int
+   - [v] (mon:monad -> acts mon -> (int -> mon.m int) -> mon.m int) -> free.m int 
 
-(** I think I would like more a refinement like this one:
-    forall x. arrow? x /\ special_tree x ==> special_tree f
-    where special_tree' returns False for Decorated. But,
-    how can one write 'arrow?'?
+   Types of programs that should not be part of MLang:
+   - [ ] how can I identify such cases?
 **)
 
-(** TODO: why is this needed? mlang_arrow should be enough **)
-instance mlang_unverified_arrow #t1 #t2 pi (d1:mlang t1) (d2:mlang t2) : mlang (unverified_arrow t1 t2 pi) =
-  { mldummy = () }
+let test_mlang_free_arrow : mlang (int -> free.m int) =
+  mlang_free_arrow mlang_int mlang_int
 
-// assume val pi : monitorable_prop
+(** Cannot be typed because universe problems
+let test_mlang_free_arrow_rhs_ho : mlang (int (int -> free.m int) -> free.m int) =
+  mlang_free_arrow free.m mlang_int (mlang_free_arrow free.m mlang_int mlang_int)
+ **)
 
-// type arr1 = unit -> MIIO unit
+let test_mlang_free_arrow_lhs_ho : mlang ((int -> free.m int) -> free.m int) =
+  mlang_free_arrow (mlang_free_arrow mlang_int mlang_int) mlang_int
 
-// val arr2 : unverified_arrow arr1 unit pi
+let test_mlang_fo_effectpoly : mlang (mon:monad -> acts mon -> int -> mon.m int) =
+  mlang_effectpoly #(fun m -> int -> m int) (mlang_free_arrow mlang_int mlang_int)
 
-// let arr2 f = Inl (f ())
+let test_mlang_lhs_ho_effectpoly : mlang (mon:monad -> acts mon -> (int -> mon.m int) -> mon.m int) =
+  mlang_effectpoly #(fun m -> (int -> m int) -> m int) (mlang_free_arrow (mlang_free_arrow mlang_int mlang_int) mlang_int)
+
+(** This can not be typed because universe problems: 
+let test_mlang_rhs_ho_effectpoly : mlang (mon:monad -> acts mon -> int -> mon.m (int -> mon.m int)) = **)
+
+let test_mlang_prog1 : mlang ((mon:monad -> acts mon -> int -> mon.m int) -> free.m int) =
+  mlang_free_arrow
+    (mlang_effectpoly #(fun m -> int -> m int) (mlang_free_arrow mlang_int mlang_int))
+    mlang_int
+
+let test_mlang_prog2 : mlang ((mon:monad -> acts mon -> (int -> mon.m int) -> mon.m int) -> free.m int) =
+  mlang_free_arrow
+    (mlang_effectpoly 
+      #(fun m -> (int -> m int) -> m int)
+      (mlang_free_arrow (mlang_free_arrow mlang_int mlang_int) mlang_int))
+    mlang_int
